10FlatMemory/MemoryFlattening.thy
@@ -28,9 +28,14 @@ primrec flatten_frame :: "(ptr \<times> nat) \<Rightarrow> nat list" where
 abbreviation flatten_stack :: "(ptr \<times> nat) list \<Rightarrow> nat list" where
   "flatten_stack sfs \<equiv> concat (map flatten_frame sfs)"
 
-primrec flatten :: "state\<^sub>v \<Rightarrow> flat_state" where
+primrec flatten :: "state\<^sub>v \<Rightarrow> state\<^sub>f" where
   "flatten (S\<^sub>v h env vs sfs) = 
-      FS (flatten_values h) (flatten_environment env) (flatten_vals vs) (flatten_stack sfs)"
+      S\<^sub>f (flatten_values h) (flatten_environment env) (flatten_vals vs) (flatten_stack sfs)"
+
+fun get_closure :: "nat heap \<Rightarrow> ptr \<Rightarrow> closure\<^sub>v" where
+  "get_closure h p = (case hlookup h p of
+      0 \<Rightarrow> Lam\<^sub>v (hlookup h (Suc p)) (hlookup h (Suc (Suc p)))
+    | Suc _ \<Rightarrow> Const\<^sub>v (hlookup h (Suc p)))"
 
 lemma [simp]: "length (flatten_closure c) = 3"
   by (induction c) simp_all
@@ -38,28 +43,48 @@ lemma [simp]: "length (flatten_closure c) = 3"
 lemma [simp]: "flatten_closure c ! 0 = (case c of Lam\<^sub>v _ _ \<Rightarrow> 0 | Const\<^sub>v _ \<Rightarrow> 1)"
   by (simp split: closure\<^sub>v.splits)
 
-lemma flatten_c1 [simp]: "flatten_closure c ! 1 = (case c of Const\<^sub>v k \<Rightarrow> k | Lam\<^sub>v p _ \<Rightarrow> 2 * p)"
+lemma flatten_c1 [simp]: "flatten_closure c ! Suc 0 = (case c of Const\<^sub>v k \<Rightarrow> k | Lam\<^sub>v p _ \<Rightarrow> 2 * p)"
   by (simp split: closure\<^sub>v.splits)
 
-lemma flatten_c2 [simp]: "flatten_closure c ! 2 = (case c of Const\<^sub>v k \<Rightarrow> 0 | Lam\<^sub>v _ pc \<Rightarrow> pc)"
+lemma flatten_c2 [simp]: "flatten_closure c ! Suc (Suc 0) = 
+    (case c of Const\<^sub>v k \<Rightarrow> 0 | Lam\<^sub>v _ pc \<Rightarrow> pc)"
   by (simp split: closure\<^sub>v.splits)
 
 lemma [simp]: "hcontains h v \<Longrightarrow> 
-  get_closure (flatten_values h) (3 * v) = flatten_closure' (hlookup h v)"
+  hlookup (flatten_values h) (3 * v) = (case hlookup h v of Lam\<^sub>v _ _ \<Rightarrow> 0 | Const\<^sub>v _ \<Rightarrow> 1)"
 proof -
   assume "hcontains h v"
-  hence H: "\<And>k g. (\<And>a. flatten_closure a ! k = g a) \<Longrightarrow>
-    k < 3 \<Longrightarrow> hlookup (hsplay flatten_closure h) (k + 3 * v) = g (hlookup h v)" by simp
-  hence "hlookup (hsplay flatten_closure h) (3 * v) = 
-    (case hlookup h v of Lam\<^sub>v _ _ \<Rightarrow> 0 | Const\<^sub>v _ \<Rightarrow> 1)" by force
-  moreover from H have "hlookup (hsplay flatten_closure h) (Suc (3 * v)) = 
-    (case hlookup h v of Lam\<^sub>v p _ \<Rightarrow> 2 * p | Const\<^sub>v k \<Rightarrow> k)"
-      by (metis flatten_c1 one_less_numeral_iff plus_1_eq_Suc semiring_norm(77))
-  moreover from H have "hlookup (hsplay flatten_closure h) (Suc (Suc (3 * v))) = 
-    (case hlookup h v of Lam\<^sub>v _ pc \<Rightarrow> pc | Const\<^sub>v k \<Rightarrow> 0)"
-      by (metis flatten_c2 add.left_neutral add_2_eq_Suc' add_Suc eval_nat_numeral(3) lessI)
-  ultimately show ?thesis by (simp split: closure\<^sub>v.splits)
+  moreover have "\<And>a. length (flatten_closure a) = 3 \<and> 
+    flatten_closure a ! 0 = (case a of Lam\<^sub>v _ _ \<Rightarrow> 0 | Const\<^sub>v _ \<Rightarrow> 1)" 
+      by (simp split: closure\<^sub>v.splits)
+  ultimately show ?thesis by (metis hlookup_hsplay zero_less_numeral add_0)
 qed
+
+lemma [simp]: "hcontains h v \<Longrightarrow> hlookup (flatten_values h) (Suc (3 * v)) = 
+  (case hlookup h v of Lam\<^sub>v p\<^sub>\<Delta> _ \<Rightarrow> 2 * p\<^sub>\<Delta> | Const\<^sub>v n \<Rightarrow> n)"
+proof -
+  assume "hcontains h v"
+  moreover have "(1::nat) < 3" by simp
+  moreover have "\<And>a. length (flatten_closure a) = 3 \<and> 
+    flatten_closure a ! 1 = (case a of Lam\<^sub>v p\<^sub>\<Delta> _ \<Rightarrow> 2 * p\<^sub>\<Delta> | Const\<^sub>v n \<Rightarrow> n)" 
+      by (simp split: closure\<^sub>v.splits)
+  ultimately show ?thesis by (metis hlookup_hsplay plus_1_eq_Suc)
+qed
+
+lemma [simp]: "hcontains h v \<Longrightarrow> hlookup (flatten_values h) (Suc (Suc (3 * v))) = 
+  (case hlookup h v of Lam\<^sub>v _ p\<^sub>\<C> \<Rightarrow> p\<^sub>\<C> | Const\<^sub>v _ \<Rightarrow> 0)"
+proof -
+  assume "hcontains h v"
+  moreover have "(2::nat) < 3" by simp
+  moreover have "\<And>a. length (flatten_closure a) = 3 \<and> 
+    flatten_closure a ! 2 = (case a of Lam\<^sub>v _ p\<^sub>\<C> \<Rightarrow> p\<^sub>\<C> | Const\<^sub>v _ \<Rightarrow> 0)" 
+      by (simp split: closure\<^sub>v.splits)
+  ultimately show ?thesis by (metis hlookup_hsplay plus_1_eq_Suc Suc_1 add_Suc)
+qed
+
+lemma [simp]: "hcontains h v \<Longrightarrow> 
+    get_closure (flatten_values h) (3 * v) = flatten_closure' (hlookup h v)"
+  by (simp split: closure\<^sub>v.splits)
 
 lemma [dest]: "hcontains h v \<Longrightarrow> get_closure (flatten_values h) (3 * v) = Const\<^sub>v k \<Longrightarrow> 
     hlookup h v = Const\<^sub>v k"
@@ -109,7 +134,7 @@ lemma flatten_halloc [simp]: "halloc h c = (h', v) \<Longrightarrow>
 lemma flatten_lt_3: "hcontains h x \<Longrightarrow> flatten_values h = H h' hp \<Longrightarrow> Suc (3 * x) < hp"
   by simp
 
-lemma [dest]: "FS h env vs sfs = flatten \<Sigma>\<^sub>c\<^sub>e \<Longrightarrow> \<exists>h\<^sub>c\<^sub>e env\<^sub>c\<^sub>e vs\<^sub>c\<^sub>e sfs\<^sub>c\<^sub>e. \<Sigma>\<^sub>c\<^sub>e = S\<^sub>v h\<^sub>c\<^sub>e env\<^sub>c\<^sub>e vs\<^sub>c\<^sub>e sfs\<^sub>c\<^sub>e \<and> 
+lemma [dest]: "S\<^sub>f h env vs sfs = flatten \<Sigma>\<^sub>c\<^sub>e \<Longrightarrow> \<exists>h\<^sub>c\<^sub>e env\<^sub>c\<^sub>e vs\<^sub>c\<^sub>e sfs\<^sub>c\<^sub>e. \<Sigma>\<^sub>c\<^sub>e = S\<^sub>v h\<^sub>c\<^sub>e env\<^sub>c\<^sub>e vs\<^sub>c\<^sub>e sfs\<^sub>c\<^sub>e \<and> 
   h = flatten_values h\<^sub>c\<^sub>e \<and> env = flatten_environment env\<^sub>c\<^sub>e \<and> vs = flatten_vals vs\<^sub>c\<^sub>e \<and> 
     sfs = flatten_stack sfs\<^sub>c\<^sub>e"
   by (induction \<Sigma>\<^sub>c\<^sub>e) simp_all
@@ -141,83 +166,87 @@ qed
 
 theorem correctf: "cd \<tturnstile> flatten \<Sigma>\<^sub>c\<^sub>e \<leadsto>\<^sub>f \<Sigma>\<^sub>f' \<Longrightarrow> chained_state \<Sigma>\<^sub>c\<^sub>e \<Longrightarrow> 
   \<exists>\<Sigma>\<^sub>c\<^sub>e'. (cd \<tturnstile> \<Sigma>\<^sub>c\<^sub>e \<leadsto>\<^sub>v \<Sigma>\<^sub>c\<^sub>e') \<and> flatten \<Sigma>\<^sub>c\<^sub>e' = \<Sigma>\<^sub>f'" 
-proof (induction "flatten \<Sigma>\<^sub>c\<^sub>e" \<Sigma>\<^sub>f' rule: evalf.induct)
-  case (evf_lookup cd pc x env p v h vs sfs)
+proof (induction "flatten \<Sigma>\<^sub>c\<^sub>e" \<Sigma>\<^sub>f' rule: eval\<^sub>f.induct)
+  case (ev\<^sub>f_lookup cd pc x env p v h vs sfs)
   then obtain h\<^sub>c\<^sub>e env\<^sub>c\<^sub>e vs\<^sub>c\<^sub>e p\<^sub>c\<^sub>e sfs\<^sub>c\<^sub>e where S: "\<Sigma>\<^sub>c\<^sub>e = S\<^sub>v h\<^sub>c\<^sub>e env\<^sub>c\<^sub>e vs\<^sub>c\<^sub>e ((p\<^sub>c\<^sub>e, Suc pc) # sfs\<^sub>c\<^sub>e) \<and> 
     h = flatten_values h\<^sub>c\<^sub>e \<and> env = flatten_environment env\<^sub>c\<^sub>e \<and> vs = flatten_vals vs\<^sub>c\<^sub>e \<and> 
       sfs = flatten_stack sfs\<^sub>c\<^sub>e \<and> p = 2 * p\<^sub>c\<^sub>e" by fastforce
-  with evf_lookup obtain v\<^sub>c\<^sub>e where V: "chain_lookup env\<^sub>c\<^sub>e p\<^sub>c\<^sub>e x = Some v\<^sub>c\<^sub>e \<and> v = 3 * v\<^sub>c\<^sub>e" by fastforce
+  with ev\<^sub>f_lookup obtain v\<^sub>c\<^sub>e where V: "chain_lookup env\<^sub>c\<^sub>e p\<^sub>c\<^sub>e x = Some v\<^sub>c\<^sub>e \<and> v = 3 * v\<^sub>c\<^sub>e" by fastforce
   with S have X: "flatten (S\<^sub>v h\<^sub>c\<^sub>e env\<^sub>c\<^sub>e (v\<^sub>c\<^sub>e # vs\<^sub>c\<^sub>e) ((p\<^sub>c\<^sub>e, pc) # sfs\<^sub>c\<^sub>e)) = 
-    FS h env (v # vs) (pc # p # sfs)" by simp
-  from evf_lookup V have "cd \<tturnstile> S\<^sub>v h\<^sub>c\<^sub>e env\<^sub>c\<^sub>e vs\<^sub>c\<^sub>e ((p\<^sub>c\<^sub>e, Suc pc) # sfs\<^sub>c\<^sub>e) \<leadsto>\<^sub>v 
+    S\<^sub>f h env (v # vs) (pc # p # sfs)" by simp
+  from ev\<^sub>f_lookup V have "cd \<tturnstile> S\<^sub>v h\<^sub>c\<^sub>e env\<^sub>c\<^sub>e vs\<^sub>c\<^sub>e ((p\<^sub>c\<^sub>e, Suc pc) # sfs\<^sub>c\<^sub>e) \<leadsto>\<^sub>v 
     S\<^sub>v h\<^sub>c\<^sub>e env\<^sub>c\<^sub>e (v\<^sub>c\<^sub>e # vs\<^sub>c\<^sub>e) ((p\<^sub>c\<^sub>e, pc) # sfs\<^sub>c\<^sub>e)" by simp
   with S X show ?case by blast
 next
-  case (evf_pushcon cd pc k h h' v env vs p sfs)
+  case (ev\<^sub>f_pushcon cd pc k h h' v env vs p sfs)
   then obtain h\<^sub>c\<^sub>e env\<^sub>c\<^sub>e vs\<^sub>c\<^sub>e p\<^sub>c\<^sub>e sfs\<^sub>c\<^sub>e where S: "\<Sigma>\<^sub>c\<^sub>e = S\<^sub>v h\<^sub>c\<^sub>e env\<^sub>c\<^sub>e vs\<^sub>c\<^sub>e ((p\<^sub>c\<^sub>e, Suc pc) # sfs\<^sub>c\<^sub>e) \<and> 
     h = flatten_values h\<^sub>c\<^sub>e \<and> env = flatten_environment env\<^sub>c\<^sub>e \<and> vs = flatten_vals vs\<^sub>c\<^sub>e \<and> 
       sfs = flatten_stack sfs\<^sub>c\<^sub>e \<and> p = 2 * p\<^sub>c\<^sub>e" by fastforce
-  with evf_pushcon have "halloc_list (hsplay flatten_closure h\<^sub>c\<^sub>e) (flatten_closure (Const\<^sub>v k)) = 
+  with ev\<^sub>f_pushcon have "halloc_list (hsplay flatten_closure h\<^sub>c\<^sub>e) (flatten_closure (Const\<^sub>v k)) = 
     (h', v)" by simp
   then obtain h\<^sub>c\<^sub>e' v\<^sub>c\<^sub>e where H: "h' = hsplay flatten_closure h\<^sub>c\<^sub>e' \<and> v = 3 * v\<^sub>c\<^sub>e \<and> 
     halloc h\<^sub>c\<^sub>e (Const\<^sub>v k) = (h\<^sub>c\<^sub>e', v\<^sub>c\<^sub>e)" by fastforce
   with S have X: "flatten (S\<^sub>v h\<^sub>c\<^sub>e' env\<^sub>c\<^sub>e (v\<^sub>c\<^sub>e # vs\<^sub>c\<^sub>e) ((p\<^sub>c\<^sub>e, pc) # sfs\<^sub>c\<^sub>e)) = 
-    FS h' env (v # vs) (pc # p # sfs)" by simp
-  from evf_pushcon H have "cd \<tturnstile> S\<^sub>v h\<^sub>c\<^sub>e env\<^sub>c\<^sub>e vs\<^sub>c\<^sub>e ((p\<^sub>c\<^sub>e, Suc pc) # sfs\<^sub>c\<^sub>e) \<leadsto>\<^sub>v 
+    S\<^sub>f h' env (v # vs) (pc # p # sfs)" by simp
+  from ev\<^sub>f_pushcon H have "cd \<tturnstile> S\<^sub>v h\<^sub>c\<^sub>e env\<^sub>c\<^sub>e vs\<^sub>c\<^sub>e ((p\<^sub>c\<^sub>e, Suc pc) # sfs\<^sub>c\<^sub>e) \<leadsto>\<^sub>v 
     S\<^sub>v h\<^sub>c\<^sub>e' env\<^sub>c\<^sub>e (v\<^sub>c\<^sub>e # vs\<^sub>c\<^sub>e) ((p\<^sub>c\<^sub>e, pc) # sfs\<^sub>c\<^sub>e)" by simp
   with S X show ?case by blast
 next
-  case (evf_pushlam cd pc pc' h p h' v env vs sfs)
+  case (ev\<^sub>f_pushlam cd pc pc' h p h' v env vs sfs)
   then obtain h\<^sub>c\<^sub>e env\<^sub>c\<^sub>e vs\<^sub>c\<^sub>e p\<^sub>c\<^sub>e sfs\<^sub>c\<^sub>e where S: "\<Sigma>\<^sub>c\<^sub>e = S\<^sub>v h\<^sub>c\<^sub>e env\<^sub>c\<^sub>e vs\<^sub>c\<^sub>e ((p\<^sub>c\<^sub>e, Suc pc) # sfs\<^sub>c\<^sub>e) \<and> 
     h = flatten_values h\<^sub>c\<^sub>e \<and> env = flatten_environment env\<^sub>c\<^sub>e \<and> vs = flatten_vals vs\<^sub>c\<^sub>e \<and> 
       sfs = flatten_stack sfs\<^sub>c\<^sub>e \<and> p = 2 * p\<^sub>c\<^sub>e" by fastforce
-  with evf_pushlam have "halloc_list (hsplay flatten_closure h\<^sub>c\<^sub>e) (flatten_closure (Lam\<^sub>v p\<^sub>c\<^sub>e pc')) = 
+  with ev\<^sub>f_pushlam have "halloc_list (hsplay flatten_closure h\<^sub>c\<^sub>e) (flatten_closure (Lam\<^sub>v p\<^sub>c\<^sub>e pc')) = 
     (h', v)" by simp
   then obtain h\<^sub>c\<^sub>e' v\<^sub>c\<^sub>e where H: "h' = hsplay flatten_closure h\<^sub>c\<^sub>e' \<and> v = 3 * v\<^sub>c\<^sub>e \<and> 
     halloc h\<^sub>c\<^sub>e (Lam\<^sub>v p\<^sub>c\<^sub>e pc') = (h\<^sub>c\<^sub>e', v\<^sub>c\<^sub>e)" by fastforce
   with S have X: "flatten (S\<^sub>v h\<^sub>c\<^sub>e' env\<^sub>c\<^sub>e (v\<^sub>c\<^sub>e # vs\<^sub>c\<^sub>e) ((p\<^sub>c\<^sub>e, pc) # sfs\<^sub>c\<^sub>e)) = 
-    FS h' env (v # vs) (pc # p # sfs)" by simp
-  from evf_pushlam S H have "cd \<tturnstile> S\<^sub>v h\<^sub>c\<^sub>e env\<^sub>c\<^sub>e vs\<^sub>c\<^sub>e ((p\<^sub>c\<^sub>e, Suc pc) # sfs\<^sub>c\<^sub>e) \<leadsto>\<^sub>v 
+    S\<^sub>f h' env (v # vs) (pc # p # sfs)" by simp
+  from ev\<^sub>f_pushlam S H have "cd \<tturnstile> S\<^sub>v h\<^sub>c\<^sub>e env\<^sub>c\<^sub>e vs\<^sub>c\<^sub>e ((p\<^sub>c\<^sub>e, Suc pc) # sfs\<^sub>c\<^sub>e) \<leadsto>\<^sub>v 
     S\<^sub>v h\<^sub>c\<^sub>e' env\<^sub>c\<^sub>e (v\<^sub>c\<^sub>e # vs\<^sub>c\<^sub>e) ((p\<^sub>c\<^sub>e, pc) # sfs\<^sub>c\<^sub>e)" by simp
   with S X show ?case by blast
 next
-  case (evf_apply cd pc h v2 p' pc' env v1 env' p2 vs p sfs)
+  case (ev\<^sub>f_apply cd pc h v2 env v1 env' p2 vs p sfs)
   then obtain h\<^sub>c\<^sub>e env\<^sub>c\<^sub>e v1\<^sub>c\<^sub>e v2\<^sub>c\<^sub>e vs\<^sub>c\<^sub>e p\<^sub>c\<^sub>e sfs\<^sub>c\<^sub>e where S: "
     \<Sigma>\<^sub>c\<^sub>e = S\<^sub>v h\<^sub>c\<^sub>e env\<^sub>c\<^sub>e (v1\<^sub>c\<^sub>e # v2\<^sub>c\<^sub>e # vs\<^sub>c\<^sub>e) ((p\<^sub>c\<^sub>e, Suc pc) # sfs\<^sub>c\<^sub>e) \<and> h = flatten_values h\<^sub>c\<^sub>e \<and> 
       env = flatten_environment env\<^sub>c\<^sub>e \<and> v1 = 3 * v1\<^sub>c\<^sub>e \<and> v2 = 3 * v2\<^sub>c\<^sub>e \<and> vs = flatten_vals vs\<^sub>c\<^sub>e \<and> 
         sfs = flatten_stack sfs\<^sub>c\<^sub>e \<and> p = 2 * p\<^sub>c\<^sub>e" by fastforce
-  with evf_apply have "get_closure (flatten_values h\<^sub>c\<^sub>e) (3 * v2\<^sub>c\<^sub>e) = Lam\<^sub>v p' pc'" by simp
-  moreover from evf_apply S have "hcontains h\<^sub>c\<^sub>e v2\<^sub>c\<^sub>e" by simp
-  ultimately obtain p\<^sub>c\<^sub>e' where P: "hlookup h\<^sub>c\<^sub>e v2\<^sub>c\<^sub>e = Lam\<^sub>v p\<^sub>c\<^sub>e' pc' \<and> p' = 2 * p\<^sub>c\<^sub>e'" by blast
+  let ?p' = "hlookup (flatten_values h\<^sub>c\<^sub>e) (Suc (3 * v2\<^sub>c\<^sub>e))"
+  let ?pc' = "hlookup (flatten_values h\<^sub>c\<^sub>e) (Suc (Suc (3 * v2\<^sub>c\<^sub>e)))"
+  from ev\<^sub>f_apply S have "get_closure (flatten_values h\<^sub>c\<^sub>e) (3 * v2\<^sub>c\<^sub>e) = Lam\<^sub>v ?p' ?pc'" by simp
+  moreover from ev\<^sub>f_apply S have "hcontains h\<^sub>c\<^sub>e v2\<^sub>c\<^sub>e" by simp
+  ultimately obtain p\<^sub>c\<^sub>e' where P: "hlookup h\<^sub>c\<^sub>e v2\<^sub>c\<^sub>e = Lam\<^sub>v p\<^sub>c\<^sub>e' ?pc' \<and> ?p' = 2 * p\<^sub>c\<^sub>e'" by blast
   obtain env\<^sub>c\<^sub>e' p2\<^sub>c\<^sub>e where E: "halloc env\<^sub>c\<^sub>e (v1\<^sub>c\<^sub>e, p\<^sub>c\<^sub>e') = (env\<^sub>c\<^sub>e', p2\<^sub>c\<^sub>e)" by fastforce
-  with evf_apply S P have X: "flatten (S\<^sub>v h\<^sub>c\<^sub>e env\<^sub>c\<^sub>e' vs\<^sub>c\<^sub>e ((Suc p2\<^sub>c\<^sub>e, pc') # (p\<^sub>c\<^sub>e, pc) # sfs\<^sub>c\<^sub>e)) = 
-    FS h env' vs (pc' # Suc (Suc p2) # pc # p # sfs)" by simp
-  from evf_apply P E have "cd \<tturnstile> S\<^sub>v h\<^sub>c\<^sub>e env\<^sub>c\<^sub>e (v1\<^sub>c\<^sub>e # v2\<^sub>c\<^sub>e # vs\<^sub>c\<^sub>e) ((p\<^sub>c\<^sub>e, Suc pc) # sfs\<^sub>c\<^sub>e) \<leadsto>\<^sub>v 
-    S\<^sub>v h\<^sub>c\<^sub>e env\<^sub>c\<^sub>e' vs\<^sub>c\<^sub>e ((Suc p2\<^sub>c\<^sub>e, pc') # (p\<^sub>c\<^sub>e, pc) # sfs\<^sub>c\<^sub>e)" by simp
+  with ev\<^sub>f_apply S P have X: "flatten (S\<^sub>v h\<^sub>c\<^sub>e env\<^sub>c\<^sub>e' vs\<^sub>c\<^sub>e ((Suc p2\<^sub>c\<^sub>e, ?pc') # (p\<^sub>c\<^sub>e, pc) # sfs\<^sub>c\<^sub>e)) = 
+    S\<^sub>f h env' vs (?pc' # Suc (Suc p2) # pc # p # sfs)" by simp
+  from ev\<^sub>f_apply P E have "cd \<tturnstile> S\<^sub>v h\<^sub>c\<^sub>e env\<^sub>c\<^sub>e (v1\<^sub>c\<^sub>e # v2\<^sub>c\<^sub>e # vs\<^sub>c\<^sub>e) ((p\<^sub>c\<^sub>e, Suc pc) # sfs\<^sub>c\<^sub>e) \<leadsto>\<^sub>v 
+    S\<^sub>v h\<^sub>c\<^sub>e env\<^sub>c\<^sub>e' vs\<^sub>c\<^sub>e ((Suc p2\<^sub>c\<^sub>e, ?pc') # (p\<^sub>c\<^sub>e, pc) # sfs\<^sub>c\<^sub>e)" by simp
   with S X show ?case by blast
 next
-  case (evf_return cd pc h env vs p sfs)
+  case (ev\<^sub>f_return cd pc h env vs p sfs)
   then obtain h\<^sub>c\<^sub>e env\<^sub>c\<^sub>e vs\<^sub>c\<^sub>e p\<^sub>c\<^sub>e sfs\<^sub>c\<^sub>e where S: "\<Sigma>\<^sub>c\<^sub>e = S\<^sub>v h\<^sub>c\<^sub>e env\<^sub>c\<^sub>e vs\<^sub>c\<^sub>e ((p\<^sub>c\<^sub>e, Suc pc) # sfs\<^sub>c\<^sub>e) \<and> 
     h = flatten_values h\<^sub>c\<^sub>e \<and> env = flatten_environment env\<^sub>c\<^sub>e \<and> vs = flatten_vals vs\<^sub>c\<^sub>e \<and> 
       sfs = flatten_stack sfs\<^sub>c\<^sub>e \<and> p = 2 * p\<^sub>c\<^sub>e" by fastforce
-  hence X: "flatten (S\<^sub>v h\<^sub>c\<^sub>e env\<^sub>c\<^sub>e vs\<^sub>c\<^sub>e sfs\<^sub>c\<^sub>e) = FS h env vs sfs" by simp
-  from evf_return have "cd \<tturnstile> S\<^sub>v h\<^sub>c\<^sub>e env\<^sub>c\<^sub>e vs\<^sub>c\<^sub>e ((p\<^sub>c\<^sub>e, Suc pc) # sfs\<^sub>c\<^sub>e) \<leadsto>\<^sub>v 
+  hence X: "flatten (S\<^sub>v h\<^sub>c\<^sub>e env\<^sub>c\<^sub>e vs\<^sub>c\<^sub>e sfs\<^sub>c\<^sub>e) = S\<^sub>f h env vs sfs" by simp
+  from ev\<^sub>f_return have "cd \<tturnstile> S\<^sub>v h\<^sub>c\<^sub>e env\<^sub>c\<^sub>e vs\<^sub>c\<^sub>e ((p\<^sub>c\<^sub>e, Suc pc) # sfs\<^sub>c\<^sub>e) \<leadsto>\<^sub>v 
     S\<^sub>v h\<^sub>c\<^sub>e env\<^sub>c\<^sub>e vs\<^sub>c\<^sub>e sfs\<^sub>c\<^sub>e" by simp
   with S X show ?case by blast
 next
-  case (evf_jump cd pc h v2 p' pc' env v1 env' p2 vs p sfs)
+  case (ev\<^sub>f_jump cd pc h v2 env v1 env' p2 vs p sfs)
   then obtain h\<^sub>c\<^sub>e env\<^sub>c\<^sub>e v1\<^sub>c\<^sub>e v2\<^sub>c\<^sub>e vs\<^sub>c\<^sub>e p\<^sub>c\<^sub>e sfs\<^sub>c\<^sub>e where S: "
     \<Sigma>\<^sub>c\<^sub>e = S\<^sub>v h\<^sub>c\<^sub>e env\<^sub>c\<^sub>e (v1\<^sub>c\<^sub>e # v2\<^sub>c\<^sub>e # vs\<^sub>c\<^sub>e) ((p\<^sub>c\<^sub>e, Suc pc) # sfs\<^sub>c\<^sub>e) \<and> h = flatten_values h\<^sub>c\<^sub>e \<and> 
       env = flatten_environment env\<^sub>c\<^sub>e \<and> v1 = 3 * v1\<^sub>c\<^sub>e \<and> v2 = 3 * v2\<^sub>c\<^sub>e \<and> vs = flatten_vals vs\<^sub>c\<^sub>e \<and> 
         sfs = flatten_stack sfs\<^sub>c\<^sub>e \<and> p = 2 * p\<^sub>c\<^sub>e" by fastforce
-  with evf_jump have "get_closure (flatten_values h\<^sub>c\<^sub>e) (3 * v2\<^sub>c\<^sub>e) = Lam\<^sub>v p' pc'" by simp
-  moreover from evf_jump S have "hcontains h\<^sub>c\<^sub>e v2\<^sub>c\<^sub>e" by simp
-  ultimately obtain p\<^sub>c\<^sub>e' where P: "hlookup h\<^sub>c\<^sub>e v2\<^sub>c\<^sub>e = Lam\<^sub>v p\<^sub>c\<^sub>e' pc' \<and> p' = 2 * p\<^sub>c\<^sub>e'" by blast
+  let ?p' = "hlookup (flatten_values h\<^sub>c\<^sub>e) (Suc (3 * v2\<^sub>c\<^sub>e))"
+  let ?pc' = "hlookup (flatten_values h\<^sub>c\<^sub>e) (Suc (Suc (3 * v2\<^sub>c\<^sub>e)))"
+  from ev\<^sub>f_jump S have "get_closure (flatten_values h\<^sub>c\<^sub>e) (3 * v2\<^sub>c\<^sub>e) = Lam\<^sub>v ?p' ?pc'" by simp
+  moreover from ev\<^sub>f_jump S have "hcontains h\<^sub>c\<^sub>e v2\<^sub>c\<^sub>e" by simp
+  ultimately obtain p\<^sub>c\<^sub>e' where P: "hlookup h\<^sub>c\<^sub>e v2\<^sub>c\<^sub>e = Lam\<^sub>v p\<^sub>c\<^sub>e' ?pc' \<and> ?p' = 2 * p\<^sub>c\<^sub>e'" by blast
   obtain env\<^sub>c\<^sub>e' p2\<^sub>c\<^sub>e where E: "halloc env\<^sub>c\<^sub>e (v1\<^sub>c\<^sub>e, p\<^sub>c\<^sub>e') = (env\<^sub>c\<^sub>e', p2\<^sub>c\<^sub>e)" by fastforce
-  with evf_jump S P have X: "flatten (S\<^sub>v h\<^sub>c\<^sub>e env\<^sub>c\<^sub>e' vs\<^sub>c\<^sub>e ((Suc p2\<^sub>c\<^sub>e, pc') # sfs\<^sub>c\<^sub>e)) = 
-    FS h env' vs (pc' # Suc (Suc p2) # sfs)" by simp
-  from evf_jump P E have "cd \<tturnstile> S\<^sub>v h\<^sub>c\<^sub>e env\<^sub>c\<^sub>e (v1\<^sub>c\<^sub>e # v2\<^sub>c\<^sub>e # vs\<^sub>c\<^sub>e) ((p\<^sub>c\<^sub>e, Suc pc) # sfs\<^sub>c\<^sub>e) \<leadsto>\<^sub>v 
-    S\<^sub>v h\<^sub>c\<^sub>e env\<^sub>c\<^sub>e' vs\<^sub>c\<^sub>e ((Suc p2\<^sub>c\<^sub>e, pc') # sfs\<^sub>c\<^sub>e)" by simp
+  with ev\<^sub>f_jump S P have X: "flatten (S\<^sub>v h\<^sub>c\<^sub>e env\<^sub>c\<^sub>e' vs\<^sub>c\<^sub>e ((Suc p2\<^sub>c\<^sub>e, ?pc') # sfs\<^sub>c\<^sub>e)) = 
+    S\<^sub>f h env' vs (?pc' # Suc (Suc p2) # sfs)" by simp
+  from ev\<^sub>f_jump P E have "cd \<tturnstile> S\<^sub>v h\<^sub>c\<^sub>e env\<^sub>c\<^sub>e (v1\<^sub>c\<^sub>e # v2\<^sub>c\<^sub>e # vs\<^sub>c\<^sub>e) ((p\<^sub>c\<^sub>e, Suc pc) # sfs\<^sub>c\<^sub>e) \<leadsto>\<^sub>v 
+    S\<^sub>v h\<^sub>c\<^sub>e env\<^sub>c\<^sub>e' vs\<^sub>c\<^sub>e ((Suc p2\<^sub>c\<^sub>e, ?pc') # sfs\<^sub>c\<^sub>e)" by simp
   with S X show ?case by blast
 qed
 
@@ -234,11 +263,30 @@ next
     using flatten_halloc by fastforce
   ultimately show ?case by simp
 next
-  case (ev\<^sub>v_apply cd pc h v2 p' pc' env v1 env' p'' vs p sfs)
-  thus ?case by (simp del: get_closure.simps)
+  case (ev\<^sub>v_apply \<C> p\<^sub>\<C> h v2 p' pc' env v1 env' p'' vs p\<^sub>\<Delta> sfs)
+  moreover hence "halloc_list (flatten_environment env) 
+    [3 * v1, hlookup (flatten_values h) (Suc (3 * v2))] = (flatten_environment env', 2 * p'')" 
+      by simp
+  moreover from ev\<^sub>v_apply have "hlookup (flatten_values h) (3 * v2) = 0" by simp
+  ultimately have "\<C> \<tturnstile> S\<^sub>f (flatten_values h) (flatten_environment env) 
+      (3 * v1 # 3 * v2 # flatten_vals vs) (Suc p\<^sub>\<C> # 2 * p\<^sub>\<Delta> # flatten_stack sfs) \<leadsto>\<^sub>f 
+    S\<^sub>f (flatten_values h) (flatten_environment env') (flatten_vals vs) 
+      (hlookup (flatten_values h) (Suc (Suc (3 * v2))) # Suc (Suc (2 * p'')) # p\<^sub>\<C> # 2 * p\<^sub>\<Delta> # 
+        flatten_stack sfs)"
+    by (metis ev\<^sub>f_apply)
+  with ev\<^sub>v_apply show ?case by simp
 next
-  case (ev\<^sub>v_jump cd pc h v2 p' pc' env v1 env' p'' vs p sfs)
-  thus ?case by (simp del: get_closure.simps)
+  case (ev\<^sub>v_jump \<C> p\<^sub>\<C> h v2 p' pc' env v1 env' p'' vs p\<^sub>\<Delta> sfs)
+  moreover hence "halloc_list (flatten_environment env) 
+    [3 * v1, hlookup (flatten_values h) (Suc (3 * v2))] = (flatten_environment env', 2 * p'')" 
+      by simp
+  moreover from ev\<^sub>v_jump have "hlookup (flatten_values h) (3 * v2) = 0" by simp
+  ultimately have "\<C> \<tturnstile> S\<^sub>f (flatten_values h) (flatten_environment env) 
+      (3 * v1 # 3 * v2 # flatten_vals vs) (Suc p\<^sub>\<C> # 2 * p\<^sub>\<Delta> # flatten_stack sfs) \<leadsto>\<^sub>f 
+    S\<^sub>f (flatten_values h) (flatten_environment env') (flatten_vals vs) 
+      (hlookup (flatten_values h) (Suc (Suc (3 * v2))) # Suc (Suc (2 * p'')) # flatten_stack sfs)"
+    by (metis ev\<^sub>f_jump)
+  with ev\<^sub>v_jump show ?case by simp
 qed fastforce+
 
 lemma completef_iter [simp]: "iter (\<tturnstile> cd \<leadsto>\<^sub>v) \<Sigma>\<^sub>c\<^sub>e \<Sigma>\<^sub>c\<^sub>e' \<Longrightarrow> chained_state \<Sigma>\<^sub>c\<^sub>e \<Longrightarrow>
